typeclass/typing/typeclass_env_mapScript.sml
@@ -1,0 +1,881 @@
+(* concrete data structures for implementing
+* instance map and type class map *)
+open HolKernel Parse boolLib bossLib dep_rewrite BasicProvers;
+open relationTheory set_relationTheory;
+open pairTheory optionTheory listTheory pred_setTheory finite_mapTheory;
+open miscTheory typeclass_typesTheory typeclass_tcexpTheory;
+open monadsyntax;
+
+val _ = new_theory "typeclass_env_map";
+
+val _ = monadsyntax.enable_monadsyntax();
+val _ = monadsyntax.enable_monad "option";
+
+Type minImplAST = ``:(mlstring list) list``; (* DNF of function names*)
+
+Datatype:
+  classinfo =
+    <| super : mlstring list
+     ; kind : Kind option
+     ; methodsig : cvname |-> PredType
+     ; minImp : minImplAST
+     ; defaults : cvname |-> tcexp |>
+End
+
+Definition super_reachable_def:
+  super_reachable cdb =
+    TC (\src dst.
+      ∃c. FLOOKUP cdb src = SOME (c:classinfo) ∧
+      MEM dst c.super)
+End
+
+Theorem super_reachable_RULES:
+  (∀x y c. FLOOKUP cdb x = SOME c ∧ MEM y c.super ⇒
+    super_reachable cdb x y) ∧
+  (∀x y z. super_reachable cdb x y ∧ super_reachable cdb y z ⇒
+    super_reachable cdb x z)
+Proof
+  rw[super_reachable_def,relationTheory.TC_RULES] >>
+  metis_tac[cj 2 relationTheory.TC_RULES]
+QED
+
+Theorem super_reachable_SUBSET = cj 1 super_reachable_RULES;
+Theorem super_reachable_trans = cj 2 super_reachable_RULES;
+
+Theorem super_reachable_LEFT1_I:
+  ∀x y z c.
+    FLOOKUP cdb x = SOME c ∧ MEM y c.super ∧
+    super_reachable cdb y z ⇒
+    super_reachable cdb x z
+Proof
+  rw[] >> irule super_reachable_trans >>
+  first_x_assum $ irule_at Any >>
+  drule_all_then irule super_reachable_SUBSET
+QED
+
+Theorem super_reachable_RIGHT1_I:
+  ∀x y z c.
+    super_reachable cdb x y ∧
+    FLOOKUP cdb y = SOME c ∧ MEM z c.super ⇒
+    super_reachable cdb x z
+Proof
+  rw[] >> irule super_reachable_trans >>
+  first_x_assum $ irule_at Any >>
+  drule_all_then irule super_reachable_SUBSET
+QED
+
+Definition super_no_cycles_def:
+  super_no_cycles cdb =
+    ∀x. ¬(super_reachable cdb x x)
+End
+
+Datatype:
+  instinfo =
+    <| cstr : (mlstring # 'b) list (* class and type variable *)
+     ; nargs : num (* number of arguments to the type constructor *)
+     ; impl : cvname |-> tcexp |> (* function name and its expression *)
+End
+
+Definition instinfo_well_scoped_def:
+  instinfo_well_scoped inf ⇔
+    (∀c v. MEM (c,v) inf.cstr ⇒ v < inf.nargs)
+End
+
+Definition instinfo_impl_ok:
+  instinfo_impl_ok cdb inst class <=>
+  ∃c. FLOOKUP cdb class = SOME c ∧
+    (∀meth ty. FLOOKUP c.methodsig meth = SOME ty ⇒
+     ∃exp.
+       FLOOKUP inst.impl meth = SOME exp ∨
+       FLOOKUP c.defaults meth = SOME exp) ∧
+    (∃minimpl. ∀m.
+      MEM minimpl c.minImp ∧ MEM m minimpl ⇒
+        ∃exp. FLOOKUP inst.impl m = SOME exp)
+End
+
+Type class_map = ``:mlstring |-> classinfo``;
+Type inst_map = ``: (mlstring # typeclass_types$ty_cons) |-> num instinfo``;
+
+Definition add_instance_def:
+  add_instance (inst_map:inst_map) cl ty info =
+    case FLOOKUP inst_map (cl,ty) of
+    | NONE => SOME $ inst_map |+ ((cl,ty), info)
+    | SOME _ => NONE
+End
+
+Definition super_keys_ok_def:
+  super_keys_ok (cl_map:class_map) =
+  (∀c clinfo c'.
+    FLOOKUP cl_map c = SOME clinfo ∧ MEM c' clinfo.super ⇒
+    ∃x. FLOOKUP cl_map c' = SOME x)
+End
+
+Definition FLOOKUP_inst_map_def:
+  FLOOKUP_inst_map inst_map c t =
+  do
+    tcons <- head_ty_cons t;
+    FLOOKUP inst_map (c,tcons)
+  od
+End
+
+(*
+Definition inst_to_types_def:
+  inst_to_PredType_scheme (inst:inst_info) =
+  (inst.nargs, (MAP (I ## TypeVar) inst.cstr),
+    (c,tcons_to_type tcons (GENLIST TypeVar inst.nargs)))
+End
+
+Definition by_inst_def:
+  by_inst inst_map c cstr t =
+    ∃tcons targs inst ts.
+      t = tcons_to_type tcons targs ∧
+      FLOOKUP inst_map (c,tcons) = SOME inst ∧
+      tsubst_inst ts (_ inst) = _ cstr (c,t)
+End
+
+Definition by_inst_def:
+  by_inst inst_map c t = OPTION_MAP SND $ lookup_inst_map inst_map c t
+End
+
+Theorem lookup_inst_map_lem:
+  ∀inst_map c t impl cstr.
+    lookup_inst_map inst_map c t = SOME (impl,cstr)
+    ⇔
+    (∃tcons targs inst_info.
+      split_ty_head t = SOME (tcons,targs) ∧
+      lookup inst_map (c,tcons) = SOME inst_info ∧
+      LENGTH targs = inst_info.nargs ∧
+      impl = inst_info.impl ∧
+      cstr = MAP (I ## (λv. EL v targs)) inst_info.cstr)
+Proof
+  reverse $ rw[lookup_inst_map_def,EQ_IMP_THM]
+  >- simp[combinTheory.C_DEF] >>
+  pairarg_tac >>
+  gvs[combinTheory.C_DEF]
+QED
+
+Theorem by_inst_lem:
+  ∀inst_map c t cstr.
+  by_inst inst_map c t = SOME cstr ⇔
+  (∃tcons targs inst_info.
+    split_ty_head t = SOME (tcons,targs) ∧
+    lookup inst_map (c,tcons) = SOME inst_info ∧
+    LENGTH targs = inst_info.nargs ∧
+      cstr = MAP (I ## (λv. EL v targs)) inst_info.cstr)
+Proof
+  simp[by_inst_def,LAMBDA_PROD,GSYM PEXISTS_THM,lookup_inst_map_lem]
+QED
+
+Theorem lookup_inst_map_thm:
+  ∀inst_map c t impl cstr.
+    lookup_inst_map inst_map c t = SOME (impl,cstr)
+    ⇔
+    (∃tcons targs inst_info.
+      split_ty_head t = SOME (tcons,targs) ∧
+      lookup inst_map (c,tcons) = SOME inst_info ∧
+      LENGTH targs = inst_info.nargs ∧
+      impl = inst_info.impl ∧
+      LENGTH cstr = LENGTH inst_info.cstr ∧
+      (∀n. n < LENGTH inst_info.cstr ⇒
+        let (cl,v) = EL n inst_info.cstr in
+          EL n cstr = (cl,EL v targs)))
+Proof
+  reverse $ rw[lookup_inst_map_lem,EQ_IMP_THM]
+  >- (
+    simp[] >>
+    irule LIST_EQ >>
+    rw[EL_MAP,oneline PAIR_MAP_THM] >>
+    CASE_TAC >>
+    first_x_assum drule >>
+    simp[]
+  ) >>
+  rw[] >>
+  pairarg_tac >>
+  gvs[EL_MAP,oneline PAIR_MAP_THM]
+QED
+
+Theorem by_inst_thm:
+  ∀inst_map c t cstr.
+    by_inst inst_map c t = SOME cstr ⇔
+    (∃tcons targs inst_info.
+      split_ty_head t = SOME (tcons,targs) ∧
+      lookup inst_map (c,tcons) = SOME inst_info ∧
+      LENGTH targs = inst_info.nargs ∧
+      LENGTH cstr = LENGTH inst_info.cstr ∧
+      (∀n. n < LENGTH inst_info.cstr ⇒
+        let (cl,v) = EL n inst_info.cstr in
+          EL n cstr = (cl,EL v targs)))
+Proof
+  simp[by_inst_def,LAMBDA_PROD,GSYM PEXISTS_THM,lookup_inst_map_thm]
+QED
+
+Inductive full_entail:
+[~mem]
+  MEM p ps ⇒ full_entail cl_map inst_map ps p
+[~super]
+  full_entail cl_map inst_map ps (c,t) ∧
+  super_reachable cl_map c s ⇒
+  full_entail cl_map inst_map ps (s,t)
+[~inst]
+  by_inst inst_map c t = SOME qs ∧
+  (∀q. MEM q qs ⇒ full_entail cl_map inst_map ps q) ⇒
+  full_entail cl_map inst_map ps (c,t)
+End
+
+Inductive entail:
+[~mem]
+  MEM p ps ⇒ entail cl_map inst_map ps p
+[~super]
+  MEM (c,t) ps ∧
+  super_reachable cl_map c s ⇒
+  entail cl_map inst_map ps (s,t)
+[~inst]
+  by_inst inst_map c t = SOME qs ∧
+  (∀q. MEM q qs ⇒ entail cl_map inst_map ps q) ⇒
+  entail cl_map inst_map ps (c,t)
+End
+
+Theorem split_ty_head_tsubst:
+  ∀t tcons targs ts.
+    split_ty_head t = SOME (tcons,targs) ⇒
+    split_ty_head (tsubst ts t) = SOME (tcons, MAP (tsubst ts) targs)
+Proof
+  ho_match_mp_tac head_ty_cons_ind >>
+  rw[] >>
+  gvs[subst_db_def,split_ty_head_thm,head_ty_cons_def,ty_args_alt]
+QED
+
+Definition well_scoped_inst_map_def:
+  well_scoped_inst_map inst_map =
+  (∀k inst_info c v.
+    lookup inst_map k = SOME inst_info ∧
+    MEM (c,v) inst_info.cstr ⇒
+    v < inst_info.nargs)
+End
+
+Theorem entail_tsubst:
+  well_scoped_inst_map inst_map ⇒
+  ∀p. entail cl_map inst_map ps p ⇒
+  ∀c t ts. p = (c,t) ⇒
+  entail cl_map inst_map (MAP (λ(c',t'). (c',tsubst ts t')) ps) (c,tsubst ts t)
+Proof
+  strip_tac >>
+  ho_match_mp_tac entail_ind >>
+  rw[]
+  >- (
+    irule entail_mem >>
+    simp[MEM_MAP] >>
+    first_x_assum $ irule_at (Pos last) >>
+    simp[]
+  )
+  >- (
+    irule entail_super >>
+    simp[MEM_MAP,PULL_EXISTS] >>
+    first_assum $ irule_at (Pos last) >>
+    first_assum $ irule_at (Pos last) >>
+    simp[]
+  ) >>
+  irule entail_inst >>
+  qexists `MAP (λ(c',t'). (c',tsubst ts t')) qs` >>
+  rw[MEM_MAP]
+  >- (
+    first_x_assum $ drule_then strip_assume_tac >>
+    pairarg_tac >>
+    gvs[]
+  ) >>
+  gvs[by_inst_thm] >>
+  drule_then (irule_at (Pos hd)) split_ty_head_tsubst >>
+  rw[] >>
+  first_x_assum drule >>
+  pairarg_tac >> gvs[EL_MAP] >>
+  DEP_REWRITE_TAC[EL_MAP] >>
+  gvs[well_scoped_inst_map_def] >>
+  last_x_assum irule >>
+  simp[MEM_EL] >>
+  metis_tac[]
+QED
+
+Theorem full_entail_tsubst:
+  well_scoped_inst_map inst_map ⇒
+  ∀p. full_entail cl_map inst_map ps p ⇒
+  ∀c t ts. p = (c,t) ⇒
+  full_entail cl_map inst_map (MAP (λ(c',t'). (c',tsubst ts t')) ps) (c,tsubst ts t)
+Proof
+  strip_tac >>
+  ho_match_mp_tac full_entail_ind >>
+  rw[]
+  >- (
+    irule full_entail_mem >>
+    simp[MEM_MAP] >>
+    first_x_assum $ irule_at (Pos last) >>
+    simp[]
+  )
+  >- (
+    irule full_entail_super >>
+    simp[MEM_MAP,PULL_EXISTS] >>
+    first_assum $ irule_at (Pos last) >>
+    first_assum $ irule_at (Pos last) >>
+    simp[]
+  ) >>
+  irule full_entail_inst >>
+  qexists `MAP (λ(c',t'). (c',tsubst ts t')) qs` >>
+  rw[MEM_MAP]
+  >- (
+    first_x_assum $ drule_then strip_assume_tac >>
+    pairarg_tac >>
+    gvs[]
+  ) >>
+  gvs[by_inst_thm] >>
+  drule_then (irule_at (Pos hd)) split_ty_head_tsubst >>
+  rw[] >>
+  first_x_assum drule >>
+  pairarg_tac >> gvs[EL_MAP] >>
+  DEP_REWRITE_TAC[EL_MAP] >>
+  gvs[well_scoped_inst_map_def] >>
+  last_x_assum irule >>
+  simp[MEM_EL] >>
+  metis_tac[]
+QED
+
+Theorem head_ty_cons_cons_types:
+  ∀t targs. head_ty_cons (cons_types t targs) = head_ty_cons t
+Proof
+  Induct_on `targs` >>
+  rw[head_ty_cons_def,cons_types_def]
+QED
+
+Theorem ty_args_cons_types:
+  ∀t targs. ty_args (cons_types t targs) = ty_args t ++ targs
+Proof
+  Induct_on `targs` >>
+  rw[cons_types_def,ty_args_alt]
+QED
+
+Theorem split_ty_head_tcons_to_type:
+  split_ty_head (tcons_to_type tcons targs) = SOME (tcons, targs)
+Proof
+  Induct_on `targs` using SNOC_INDUCT >>
+  gvs[tcons_to_type_def,split_ty_head_thm] >>
+  rw[cons_types_def,ty_args_alt,head_ty_cons_def] >>
+  gvs[head_ty_cons_cons_types,ty_args_cons_types]
+QED
+
+Theorem tcons_to_type_split_ty_head:
+  ∀t tcons targs.
+    split_ty_head t = SOME (tcons,targs) ⇒
+    tcons_to_type tcons targs = t
+Proof
+  ho_match_mp_tac head_ty_cons_ind >>
+  rw[] >>
+  gvs[split_ty_head_thm,head_ty_cons_def,
+    ty_args_alt,tcons_to_type_alt] >>
+  gvs[tcons_to_type_def,cons_types_SNOC]
+QED
+
+Theorem tcons_to_type_NEQ_TypeVar:
+  ∀v. tcons_to_type tcons targs ≠ TypeVar v
+Proof
+  rpt strip_tac >>
+  pop_assum $ mp_tac o Q.AP_TERM `split_ty_head` >>
+  simp[split_ty_head_tcons_to_type,split_ty_head_thm,head_ty_cons_def]
+QED
+
+Triviality tcons_to_type_tsubst_TypeVar:
+  tcons_to_type tcons targs =
+    tsubst targs $ tcons_to_type tcons $ GENLIST TypeVar (LENGTH targs)
+Proof
+  simp[tsubst_tcons_to_type,MAP_GENLIST] >>
+  AP_TERM_TAC >>
+  PURE_REWRITE_TAC[Once $ GSYM GENLIST_ID] >>
+  irule GENLIST_CONG >>
+  simp[subst_db_def]
+QED
+
+(* `entail` is equivalent to `full_entail`
+* if for every instance in inst_map,
+* the constraint ps for the instance (c,t)
+* `entail`s (s,t) for all super class s of c *)
+Definition entail_wf_def:
+  entail_wf cl_map inst_map ⇔
+  ∀c tcons inst clinfo s.
+    FLOOKUP inst_map (c,tcons) = SOME inst ∧
+    FLOOKUP cl_map c = SOME clinfo ∧ MEM s clinfo.super ⇒
+    ∃inst'. FLOOKUP inst_map (s,tcons) = SOME inst' ∧
+    inst'.nargs = inst.nargs ∧
+    ∀cl v. MEM (cl,v) inst'.cstr ⇒
+      MEM (cl,v) inst.cstr ∨
+      ∃scl. MEM (scl,v) inst.cstr ∧ super_reachable cl_map scl cl
+End
+
+Definition inst_map_constraints_ok_def:
+  inst_map_constraints_ok cl_map inst_map ⇔
+  (∀k inst x.
+    FLOOKUP inst_map k = SOME inst ∧ MEM x inst.cstr ⇒
+      ∃clinfo. FLOOKKUP cl_map (FST x) = SOME clinfo)
+End
+
+Theorem entail_super_TypeVar:
+  well_scoped_inst_map inst_map ∧
+  lookup inst_map (c,tcons) = SOME inst ∧
+  FLOOKUP cl_map c = SOME clinfo ∧
+  MEM s clinfo.super ⇒
+  (entail cl_map inst_map (MAP (I ## TypeVar) inst.cstr)
+    (s,tcons_to_type tcons (GENLIST TypeVar inst.nargs)) ⇔
+   ∃inst'. lookup inst_map (s,tcons) = SOME inst' ∧
+    inst'.nargs = inst.nargs ∧
+    ∀cl v. MEM (cl,v) inst'.cstr ⇒
+      MEM (cl,v) inst.cstr ∨
+      ∃scl. MEM (scl,v) inst.cstr ∧ super_reachable cl_map scl cl)
+Proof
+  rw[EQ_IMP_THM]
+  >- (
+    reverse $ pop_assum $ strip_assume_tac o SRULE[Once entail_cases]
+    >- (
+      gvs[by_inst_lem,split_ty_head_tcons_to_type,MEM_MAP,PULL_EXISTS] >>
+      rw[] >>
+      `v < inst_info.nargs` by (
+        gvs[well_scoped_inst_map_def] >>
+        last_x_assum irule >>
+        metis_tac[MEM_EL]) >>
+      first_x_assum drule >>
+      rw[Once entail_cases] >>
+      gvs[MEM_MAP]
+      >- (
+        rename1 `MEM p inst.cstr` >>
+        Cases_on `p` >>
+        gvs[]
+      )
+      >- (
+        rename1 `MEM p inst.cstr` >>
+        Cases_on `p` >>
+        gvs[] >>
+        disj2_tac >>
+        metis_tac[]
+      ) >>
+      gvs[by_inst_lem,split_ty_head_thm,head_ty_cons_def]
+    ) >>
+    gvs[MEM_MAP] >>
+    rename1 `MEM p inst.cstr` >>
+    Cases_on `p` >>
+    gvs[tcons_to_type_NEQ_TypeVar]
+  ) >>
+  irule entail_inst >>
+  rw[by_inst_lem,split_ty_head_tcons_to_type,MEM_MAP,PULL_EXISTS] >>
+  rename1 `entail _ _ _ (_ p)` >>
+  Cases_on `p` >>
+  first_x_assum drule >>
+  rw[]
+  >- (
+    irule entail_mem >>
+    simp[MEM_MAP] >>
+    first_assum $ irule_at (Pos last) >>
+    DEP_REWRITE_TAC[EL_GENLIST] >>
+    gvs[well_scoped_inst_map_def] >>
+    last_x_assum irule >>
+    metis_tac[MEM_EL]
+  ) >>
+  irule entail_super >>
+  simp[MEM_MAP] >>
+  first_assum $ irule_at (Pos last) >>
+  first_assum $ irule_at (Pos last) >>
+  simp[] >>
+  DEP_REWRITE_TAC[EL_GENLIST] >>
+  gvs[well_scoped_inst_map_def] >>
+  last_x_assum irule >>
+  metis_tac[MEM_EL]
+QED
+
+Theorem entail_wf_alt:
+  well_scoped_inst_map inst_map ⇒
+  (entail_wf cl_map inst_map ⇔
+  ∀c tcons inst clinfo s.
+    lookup inst_map (c,tcons) = SOME inst ∧
+    FLOOKUP cl_map c = SOME clinfo ∧ MEM s clinfo.super ⇒
+    entail cl_map inst_map (MAP (I ## TypeVar) inst.cstr)
+      (s,tcons_to_type tcons (GENLIST TypeVar inst.nargs)))
+Proof
+  rw[entail_wf_def,EQ_IMP_THM]
+  >- (
+    first_x_assum $ drule_then $ drule_then drule >>
+    rw[] >>
+    metis_tac[entail_super_TypeVar]
+  ) >>
+  first_x_assum $ drule_then $ drule_then drule >>
+  metis_tac[entail_super_TypeVar]
+QED
+
+Triviality entail_wf_lookup_super:
+  entail_wf cl_map inst_map ∧
+  FLOOKUP cl_map c = SOME c' ∧
+  MEM s c'.super ∧
+  lookup inst_map (c,tcons) = SOME inst ⇒
+  ∃inst'. lookup inst_map (s,tcons) = SOME inst' ∧
+    inst'.nargs = inst.nargs ∧
+    ∀cl v. MEM (cl,v) inst'.cstr ⇒
+      MEM (cl,v) inst.cstr ∨
+      ∃scl. MEM (scl,v) inst.cstr ∧ super_reachable cl_map scl cl
+Proof
+  rw[] >>
+  gvs[entail_wf_def] >>
+  ntac 2 (first_x_assum drule >> rw[]) >>
+  gvs[]
+QED
+
+Theorem entail_wf_lookup_super_reachable:
+  entail_wf cl_map inst_map ⇒
+  ∀c s. super_reachable cl_map c s ⇒
+  ∀tcons inst. lookup inst_map (c,tcons) = SOME inst ⇒
+  ∃inst'. lookup inst_map (s,tcons) = SOME inst' ∧
+    inst'.nargs = inst.nargs ∧
+    ∀cl v. MEM (cl,v) inst'.cstr ⇒
+      MEM (cl,v) inst.cstr ∨
+      ∃scl. MEM (scl,v) inst.cstr ∧ super_reachable cl_map scl cl
+Proof
+  strip_tac >>
+  simp[Once super_reachable_def] >>
+  ho_match_mp_tac TC_INDUCT_LEFT1 >>
+  rw[]
+  >- metis_tac[entail_wf_lookup_super] >>
+  drule_all entail_wf_lookup_super >>
+  rw[] >>
+  last_x_assum drule >> rw[] >>
+  rw[] >>
+  first_x_assum drule >> rw[] >>
+  first_x_assum drule >> rw[]
+  >- metis_tac[] >>
+  disj2_tac >>
+  irule_at (Pos last) super_reachable_trans >>
+  metis_tac[]
+QED
+
+Theorem entail_strong_ind:
+  ∀cl_map inst_map ps entail'.
+    (∀p. MEM p ps ⇒ entail' p) ∧
+    (∀c s t.
+      MEM (c,t) ps ∧ super_reachable cl_map c s ⇒ entail' (s,t)) ∧
+    (∀c qs t.
+      by_inst inst_map c t = SOME qs ∧ (∀q. MEM q qs ⇒
+        entail cl_map inst_map ps q ∧ entail' q) ⇒
+      entail' (c,t)) ⇒
+  ∀a0. entail cl_map inst_map ps a0 ⇒ entail' a0
+Proof
+  rpt gen_tac >>
+  strip_tac >>
+  `∀a0. entail cl_map inst_map ps a0 ⇒
+    entail' a0 ∧ entail cl_map inst_map ps a0` suffices_by rw[] >>
+  ho_match_mp_tac entail_ind >>
+  rw[]
+  >- drule_all_then irule entail_mem
+  >- metis_tac[]
+  >- drule_all_then irule entail_super >>
+  irule entail_inst >>
+  rw[]
+QED
+
+Triviality entail_wf_super_reachable':
+  entail_wf cl_map inst_map ⇒
+  ∀p. entail cl_map inst_map ps p ⇒
+    ∀c t clinfo s. p = (c,t) ∧
+    (c = s ∨
+    super_reachable cl_map c s) ⇒
+    entail cl_map inst_map ps (s,t)
+Proof
+  strip_tac >>
+  ho_match_mp_tac entail_strong_ind >>
+  rw[]
+  >- drule_then irule entail_mem
+  >- drule_all_then irule entail_super
+  >- drule_all_then irule entail_super
+  >- (
+    irule entail_super >>
+    first_assum $ irule_at (Pos hd) >>
+    drule_all_then irule super_reachable_trans) >>
+  gvs[IMP_CONJ_THM,FORALL_AND_THM] >>
+  gvs[PULL_FORALL,AND_IMP_INTRO]
+  >- drule_all_then irule entail_inst >>
+  gvs[by_inst_lem,MEM_MAP,PULL_EXISTS,LAMBDA_PROD,
+    GSYM PFORALL_THM,GSYM PEXISTS_THM] >>
+  irule entail_inst >>
+  simp[by_inst_lem,MEM_MAP,
+    PULL_EXISTS,LAMBDA_PROD,GSYM PFORALL_THM] >>
+  drule_all entail_wf_lookup_super_reachable >>
+  rw[] >>
+  rw[MEM_MAP,GSYM PEXISTS_THM] >>
+  first_x_assum drule >>
+  rw[] >>
+  first_x_assum drule >> rw[]
+QED
+
+Theorem entail_wf_super_reachable:
+  ∀cl_map inst_map ps c t s.
+    entail_wf cl_map inst_map ∧
+    entail cl_map inst_map ps (c,t) ∧
+    super_reachable cl_map c s ⇒
+    entail cl_map inst_map ps (s,t)
+Proof
+  metis_tac[entail_wf_super_reachable']
+QED
+
+Theorem entail_eq_full_entail:
+  entail_wf cl_map inst_map ⇒
+  ∀p. (entail cl_map inst_map ps p ⇔ full_entail cl_map inst_map ps p)
+Proof
+  strip_tac >>
+  simp[EQ_IMP_THM,FORALL_AND_THM] >>
+  conj_tac
+  >- (
+    ho_match_mp_tac entail_ind >>
+    rw[]
+    >- drule_all_then irule full_entail_mem
+    >- (
+      drule_at_then (Pos last) irule full_entail_super >>
+      drule_then irule full_entail_mem
+    )
+    >- drule_all_then irule full_entail_inst
+  ) >>
+  ho_match_mp_tac full_entail_ind >>
+  rw[]
+  >- drule_all_then irule entail_mem
+  >- drule_all_then irule entail_wf_super_reachable
+  >- drule_all_then irule entail_inst
+QED
+
+Theorem entail_monotone:
+  ∀p. entail cl_map inst_map ps p ⇒
+  (∀q. MEM q ps ⇒ MEM q qs) ⇒
+  entail cl_map inst_map qs p
+Proof
+  ho_match_mp_tac entail_ind >>
+  rw[]
+  >- (irule entail_mem >> metis_tac[])
+  >- (irule entail_super >> metis_tac[]) >>
+  irule entail_inst >> metis_tac[]
+QED
+
+Theorem full_entail_monotone:
+  ∀p. full_entail cl_map inst_map ps p ⇒
+  (∀q. MEM q ps ⇒ MEM q qs) ⇒
+  full_entail cl_map inst_map qs p
+Proof
+  ho_match_mp_tac full_entail_ind >>
+  rw[]
+  >- (irule full_entail_mem >> metis_tac[])
+  >- (irule full_entail_super >> metis_tac[]) >>
+  irule full_entail_inst >> metis_tac[]
+QED
+
+Theorem full_entail_add_full_entail:
+  ∀p. full_entail cl_map inst_map (q::ps) p ⇒
+  full_entail cl_map inst_map ps q ⇒
+  full_entail cl_map inst_map ps p
+Proof
+  ho_match_mp_tac full_entail_ind >>
+  rw[]
+  >- simp[]
+  >- drule_then irule full_entail_mem
+  >- (irule full_entail_super >> metis_tac[]) >>
+  drule_then irule full_entail_inst >>
+  rw[]
+QED
+
+Triviality type_size_GT_0:
+  ∀t. 0 < type_size t
+Proof
+  Cases_on `t` >>
+  simp[type_size_def]
+QED
+
+Theorem type_size_tcons_to_type:
+  ∀t targs.
+  MEM t targs ⇒
+  type_size t < type_size (tcons_to_type tcons targs)
+Proof
+  Induct_on `targs` using SNOC_INDUCT >>
+  rw[tcons_to_type_SNOC,type_size_def]
+  >- rw[] >>
+  irule arithmeticTheory.LESS_TRANS >>
+  first_x_assum $ drule_then $ irule_at (Pos hd) >>
+  DECIDE_TAC
+QED
+
+(* entail_aux terminates if every q in qs is smaller than t *)
+Definition entail_aux_def:
+  (entail_aux supers inst_map (c,t) =
+    if well_scoped_inst_map inst_map
+    then
+      (EXISTS (\visited. lookup visited c = SOME t) supers ∨
+      (case by_inst inst_map c t of
+        | NONE => F
+        | SOME qs => entail_aux_list supers inst_map qs))
+    else F (* should not happen given the map is well formed *)) ∧
+
+  (entail_aux_list supers inst_map [] = T) ∧
+  (entail_aux_list supers inst_map (q::qs) =
+    (entail_aux supers inst_map q ∧
+     entail_aux_list supers inst_map qs))
+Termination
+  WF_REL_TAC `inv_image ($< LEX $<) (λx.
+    (case x of
+     | INR (_,_,qs) => list_max $ MAP (type_size o SND) qs
+     | INL (_,_,_,t) => type_size t),
+    (case x of
+     | INR (_,_,qs) => LENGTH qs
+     | INL _ => 0))` >>
+  rw[]
+  >- (
+    gvs[by_inst_lem] >>
+    PURE_REWRITE_TAC[Once $ GSYM arithmeticTheory.GREATER_DEF] >>
+    irule list_max_intro >>
+    simp[EVERY_MAP,arithmeticTheory.GREATER_DEF,type_size_GT_0] >>
+    drule_then (assume_tac o GSYM) tcons_to_type_split_ty_head >>
+    gvs[EVERY_EL] >>
+    rw[] >>
+    gvs[well_scoped_inst_map_def] >>
+    last_x_assum $ drule_then strip_assume_tac >>
+    irule type_size_tcons_to_type >>
+    Cases_on `EL n inst_info.cstr` >>
+    gvs[] >>
+    rename1 `EL n inst_info.cstr = (a,b)` >>
+    first_x_assum $ qspecl_then [`a`,`b`] mp_tac >>
+    metis_tac[MEM_EL]
+  ) >>
+  simp[GSYM arithmeticTheory.LE_LT,list_max_def]
+End
+
+Definition entail_impl_def:
+  entail_impl cl_map inst_map ps (c,t) =
+   case OPT_MMAP (by_super cl_map) ps of
+   | NONE => F
+   | SOME visiteds => entail_aux visiteds inst_map (c,t)
+End
+
+Theorem entail_aux_list_EVERY:
+  entail_aux_list supers inst_map = EVERY (entail_aux supers inst_map)
+Proof
+  rw[FUN_EQ_THM] >>
+  rename1 `entail_aux_list _ _ l` >>
+  Induct_on `l` >>
+  simp[entail_aux_def]
+QED
+
+Theorem entail_aux_induct_EVERY:
+  ∀P.
+  (∀(supers:(mlstring,type) map list) inst_map c t.
+    (∀qs q.
+      well_scoped_inst_map inst_map ∧
+      by_inst inst_map c t = SOME qs ∧ MEM q qs ⇒
+      P supers inst_map q) ⇒
+    P supers inst_map (c,t)) ⇒
+    (∀supers inst_map p. P supers inst_map p)
+Proof
+  ntac 2 strip_tac >>
+  qspecl_then [`P`,`λv0 v1 v2. ∀q. MEM q v2 ⇒ P v0 v1 q`]
+    mp_tac entail_aux_ind >>
+  impl_tac >>
+  rw[] >>
+  metis_tac[]
+QED
+
+Theorem OPT_MMAP_SOME_EL:
+  ∀l fl. OPT_MMAP f l = SOME fl ⇒
+  LENGTH fl = LENGTH l ∧
+  (∀n. n < LENGTH l ⇒ f (EL n l) = SOME (EL n fl))
+Proof
+  Induct_on `l` >>
+  rw[OPT_MMAP_def] >>
+  gvs[] >>
+  Cases_on `n` >>
+  simp[]
+QED
+
+Theorem OPT_MMAP_NONE:
+  ∀l. OPT_MMAP f l = NONE ⇒
+  ∃x. MEM x l ∧ f x = NONE
+Proof
+  Induct_on `l` >>
+  rw[OPT_MMAP_def] >>
+  metis_tac[]
+QED
+
+Theorem entail_aux_thm:
+  ∀supers inst_map p cl_map ps.
+  map_ok cl_map ∧ map_ok inst_map ∧
+  well_scoped_inst_map inst_map ∧ super_keys_ok cl_map ∧
+  (∀q. MEM q ps ⇒ ∃clinfo. lookup cl_map (FST q) = SOME clinfo) ∧
+  (LENGTH supers = LENGTH ps) ∧
+  (∀n. n < LENGTH ps ⇒
+    by_super cl_map (EL n ps) = SOME (EL n supers)) ⇒
+  (entail_aux supers inst_map p ⇔
+    entail (to_class_map cl_map) inst_map ps p)
+Proof
+  ho_match_mp_tac entail_aux_induct_EVERY >>
+  rw[] >>
+  gvs[AND_IMP_INTRO,cj 1 PULL_FORALL] >>
+  last_x_assum $ drule_at (Pos last) >>
+  rw[] >>
+  simp[entail_aux_def] >>
+  rw[EQ_IMP_THM]
+  >- (
+    gvs[EXISTS_MEM] >>
+    qpat_x_assum `MEM visited supers` $
+      strip_assume_tac o SRULE[MEM_EL] >>
+    gvs[] >>
+    first_x_assum $ drule_then assume_tac >>
+    Cases_on `EL n ps` >>
+    drule_all $ iffLR by_super_thm >>
+    rw[]
+    >- (irule entail_mem >> metis_tac[MEM_EL]) >>
+    irule entail_super >> metis_tac[MEM_EL]
+  )
+  >- (
+    pop_assum mp_tac >>
+    TOP_CASE_TAC >>
+    rw[entail_aux_list_EVERY,EVERY_MEM] >>
+    irule entail_inst >>
+    simp[]
+  ) >>
+  reverse $ pop_assum $ strip_assume_tac o SRULE[Once entail_cases]
+  >- simp[entail_aux_list_EVERY,EVERY_MEM] >>
+  qpat_x_assum `MEM _ ps` $
+    strip_assume_tac o GSYM o SRULE[MEM_EL] >>
+  first_x_assum $ drule_then assume_tac >>
+  gvs[EXISTS_MEM] >>
+  drule_then strip_assume_tac $
+    SRULE[DISJ_IMP_THM,FORALL_AND_THM] $ iffRL by_super_thm >>
+  metis_tac[MEM_EL]
+QED
+
+Theorem entail_impl_thm:
+  map_ok cl_map ∧ map_ok inst_map ∧
+  well_scoped_inst_map inst_map ∧ super_keys_ok cl_map ∧
+  (∀q. MEM q ps ⇒ ∃clinfo. lookup cl_map (FST q) = SOME clinfo) ⇒
+  entail_impl cl_map inst_map ps p =
+    entail (to_class_map cl_map) inst_map ps p
+Proof
+  rw[oneline entail_impl_def] >>
+  ntac 2 TOP_CASE_TAC
+  >- (
+    dxrule_then strip_assume_tac OPT_MMAP_NONE >>
+    first_assum $ drule_then strip_assume_tac >>
+    drule_all_then (qspec_then `SND x` mp_tac) $
+      SRULE[PULL_EXISTS] $ iffLR well_formed_by_super >>
+    rw[]
+  ) >>
+  dxrule_then strip_assume_tac OPT_MMAP_SOME_EL >>
+  irule entail_aux_thm >>
+  rw[]
+QED
+
+Theorem entail_impl_full_entail:
+  map_ok cl_map ∧ map_ok inst_map ∧
+  well_scoped_inst_map inst_map ∧ super_keys_ok cl_map ∧
+  entail_wf (to_class_map cl_map) inst_map ∧
+  (∀q. MEM q ps ⇒ ∃clinfo. lookup cl_map (FST q) = SOME clinfo) ⇒
+  entail_impl cl_map inst_map ps p =
+    full_entail (to_class_map cl_map) inst_map ps p
+Proof
+  metis_tac[entail_impl_thm,entail_eq_full_entail]
+QED
+*)
+
+val _ = export_theory();
